more

Terms_with_Bindings.thy
@@ -1,82 +1,83 @@
 theory Terms_with_Bindings
+<<<<<<< local
+imports Prelim
+=======
 imports NonFreeInput
+>>>>>>> other
 begin
 
-type_synonym var = nat type_synonym const = nat
+(* type_synonym var = nat type_synonym const = nat *)
 
-fun neq where "neq x y = (x \<noteq> y)"
-
-nonfreedata lam =
-    Ct const | V var | Ap lam lam | Lm var lam
-  | Subst lam lam var (* Subst X Y z = X[Y/z] *)
+nonfreedata ('var,'const) trm =
+    Var 'var | Ct 'const | App "('var,'const) trm" "('var,'const) trm" | Lam 'var "('var,'const) trm"
+  | subst "('var,'const) trm" "('var,'const) trm" 'var (* subst X Y z = X[Y/z] *)
 where
-  Subst_Ct: "Subst (Ct c) X x = Ct c"
-| Subst_V1: "Subst (V x) X x = X"
-| Subst_V2: "neq x y \<Longrightarrow> Subst (V x) Y y = V x"
-| Subst_Ap: "Subst (Ap X Y) Z z = Ap (Subst X Z z) (Subst Y Z z)"
-| Subst_Lm: "\<lbrakk>neq x y ; fresh x Y\<rbrakk> \<Longrightarrow> Subst (Lm x X) Y y = Lm x (Subst X Y y)"
+  subst_V1: "subst (Var x) X x = X"
+| subst_Ct: "subst (Ct c) X x = Ct c"
+| subst_V2: "neq x y \<Longrightarrow> subst (Var x) Y y = Var x"
+| subst_App: "subst (App X Y) Z z = App (subst X Z z) (subst Y Z z)"
+| subst_Lam: "\<lbrakk>neq x y ; fresh x Y\<rbrakk> \<Longrightarrow> subst (Lam x X) Y y = Lam x (subst X Y y)"
+| fresh_V: "neq x y \<Longrightarrow> fresh x (Var y)"
 | fresh_Ct: "fresh x (Ct c)"
-| fresh_V: "neq x y \<Longrightarrow> fresh x (V y)"
-| fresh_Ap: "\<lbrakk>fresh x Y ; fresh x Z\<rbrakk> \<Longrightarrow> fresh x (Ap Y Z)"
-| fresh_Lm1: "fresh x (Lm x X)"
-| fresh_Lm2: "fresh x Y \<Longrightarrow> fresh x (Lm y Y)"
-| Lm_Subst:  "\<lbrakk>neq y x ; fresh y X\<rbrakk> \<Longrightarrow> Lm y (Subst X (V y) x) = Lm x X"
+| fresh_App: "\<lbrakk>fresh x Y ; fresh x Z\<rbrakk> \<Longrightarrow> fresh x (App Y Z)"
+| fresh_Lam1: "fresh x (Lam x X)"
+| fresh_Lam2: "fresh x Y \<Longrightarrow> fresh x (Lam y Y)"
+| Lam_subst:  "\<lbrakk>neq y x ; fresh y X\<rbrakk> \<Longrightarrow> Lam y (subst X (Var y) x) = Lam x X"
+| fresh_subst: "\<lbrakk>fresh x X; fresh x Z\<rbrakk> \<Longrightarrow>  fresh x (subst X Z z)"
 
-declare Subst_Ct[simp] Subst_V1[simp] Subst_V2[simp] Subst_Ap[simp] Subst_Lm[simp]
-        fresh_Ct[simp] fresh_V[simp] fresh_Ap[simp] fresh_Lm1[simp] fresh_Lm2[simp]
-        Lm_Subst[simp]
+declare subst_V1[simp] subst_V2[simp] subst_Ct[simp] subst_App[simp] subst_Lam[simp]
+        fresh_V[simp] fresh_Ct[simp] fresh_App[simp] fresh_Lam1[simp] fresh_Lam2[simp]
+        Lam_subst[simp] fresh_subst[simp]
 
-(* Count number of free occurrences of a variable in a term: *)
+(* Count number of free occurrences of a variable in a trm: *)
 nonfreeiter
-  numoccs :: "lam \<Rightarrow> (var \<Rightarrow> nat)"
+  numoccs :: "('var,'const) trm \<Rightarrow> ('var \<Rightarrow> nat)"
 where
-  "numoccs (Ct c) = (\<lambda> z. 0)"
-| "numoccs (V x) = (\<lambda> z. if x = z then 1 else 0)"
-| "numoccs (Ap X Y)  = (\<lambda> z. numoccs X z + numoccs Y z)"
-| "numoccs (Lm x X) = (\<lambda> z. if x = z then 0 else numoccs X z)"
-| "numoccs (Subst X Y y) = (\<lambda> z.
+  "numoccs (Var x) = (\<lambda> z. if x = z then 1 else 0)"
+| "numoccs (Ct c) = (\<lambda> z. 0)"
+| "numoccs (App X Y)  = (\<lambda> z. numoccs X z + numoccs Y z)"
+| "numoccs (Lam x X) = (\<lambda> z. if x = z then 0 else numoccs X z)"
+| "numoccs (subst X Y y) = (\<lambda> z.
      if y = z then numoccs X y * numoccs Y z
      else numoccs X z + numoccs X y * numoccs Y z)"
-| "fresh interpretedas (\<lambda> x (occs :: var \<Rightarrow> nat). occs x = 0)"
+| "(fresh :: 'var \<Rightarrow> ('var,'const) trm \<Rightarrow> bool) interpretedas (\<lambda> x (occs :: 'var \<Rightarrow> nat). occs x = 0)"
 by (auto simp: algebra_simps)
 
-definition lm :: const where "lm \<equiv> 0::nat"  definition ap :: const where "ap \<equiv> Suc 0"
-definition enc_const :: "const \<Rightarrow> const" where "enc_const c = Suc (Suc c)"
+datatype 'const const = Old 'const | lam | app
 
-(* HOAS encoding of lambda terms in themselves, proved adequate at definition time! *)
+(* HOAS encoding of lambda trms in themselves, proved adequate at definition time! *)
 nonfreeiter
-  enc :: "lam \<Rightarrow> lam"
+  enc :: "('var,'const) trm \<Rightarrow> ('var,'const const) trm"
 where
-  "enc (Ct c) = Ct (enc_const c)"
-| "enc (V x) = V x"
-| "enc (Ap X Y) = Ap (Ap (Ct ap) (enc X)) (enc Y)"
-| "enc (Lm x X) = Ap (Ct lm) (Lm x (enc X))"
-| "enc (Subst X Y y) = Subst (enc X) (enc Y) y"
-| "fresh interpretedas fresh"
+  "enc (Var x) = Var x"
+| "enc (Ct c) = Ct (Old c)"
+| "enc (App X Y) = App (App (Ct app) (enc X)) (enc Y)"
+| "enc (Lam x X) = App (Ct lam) (Lam x (enc X))"
+| "enc (subst X Y y) = subst (enc X) (enc Y) y"
+| "(fresh :: 'var \<Rightarrow> ('var,'const) trm \<Rightarrow> bool) interpretedas
+   (fresh :: 'var \<Rightarrow> ('var,'const const) trm \<Rightarrow> bool)"
 by auto
 
-(* Interpretation of terms in semantic domains: *)
-typedecl dom
-consts CT :: "'const \<Rightarrow> dom"
-consts LM :: "(dom \<Rightarrow> dom) \<Rightarrow> dom"
-consts AP :: "dom \<Rightarrow> dom \<Rightarrow> dom"
+(* Interpretation of trms in semantic domains: *)
 
 locale Semantics =
-fixes CT :: "const \<Rightarrow> 'dom"
-  and LM :: "('dom \<Rightarrow> 'dom) \<Rightarrow> 'dom"
-  and AP :: "'dom \<Rightarrow> 'dom \<Rightarrow> 'dom"
+fixes APP :: "'dom \<Rightarrow> 'dom \<Rightarrow> 'dom"
+  and LAM :: "('dom \<Rightarrow> 'dom) \<Rightarrow> 'dom"
 begin
 
 nonfreeiter
-  sem :: "lam \<Rightarrow> (var \<Rightarrow> 'dom) \<Rightarrow> 'dom"
+  sem :: "('var,'const) trm \<Rightarrow> ('const \<Rightarrow> 'dom) \<Rightarrow> ('var \<Rightarrow> 'dom) \<Rightarrow> 'dom"
 where
-  "sem (Ct c) = (\<lambda> \<rho>. CT c)"
-| "sem (V x) = (\<lambda> \<rho>. \<rho> x)"
-| "sem (Ap X Y) = (\<lambda> \<rho>. AP (sem X \<rho>) (sem Y \<rho>))"
-| "sem (Lm x X) = (\<lambda> \<rho>. LM (\<lambda> d. sem X (\<rho> (x := d))))"
-| "sem (Subst X Y y) = (\<lambda> \<rho>. sem X (\<rho> (y := sem Y \<rho>)))"
-| "fresh interpretedas (\<lambda> x (K::(var \<Rightarrow> 'dom) \<Rightarrow> 'dom). \<forall> \<rho>1 \<rho>2. (\<forall> y. y \<noteq> x \<longrightarrow> \<rho>1 y = \<rho>2 y) \<longrightarrow> K \<rho>1 = K \<rho>2)"
-apply (auto intro!: ext arg_cong[of _ _ LM] arg_cong[of _ _ AP] arg_cong2[of _ _ _ _ AP])
+  "sem (Var x) = (\<lambda> \<xi> \<rho>. \<rho> x)"
+| "sem (Ct c) = (\<lambda> \<xi> \<rho>. \<xi> c)"
+| "sem (App X Y) = (\<lambda> \<xi> \<rho>. APP (sem X \<xi> \<rho>) (sem Y \<xi> \<rho>))"
+| "sem (Lam x X) = (\<lambda> \<xi> \<rho>. LAM (\<lambda> d. sem X \<xi> (\<rho> (x := d))))"
+| "sem (subst X Y y) = (\<lambda> \<xi> \<rho>. sem X \<xi> (\<rho> (y := sem Y \<xi> \<rho>)))"
+| "(fresh :: 'var \<Rightarrow> ('var,'const) trm \<Rightarrow> bool) interpretedas
+   (\<lambda> x (K :: ('const \<Rightarrow> 'dom) \<Rightarrow> ('var \<Rightarrow> 'dom) \<Rightarrow> 'dom).
+      \<forall> \<xi> \<rho>1 \<rho>2. (\<forall> y. y \<noteq> x \<longrightarrow> \<rho>1 y = \<rho>2 y) \<longrightarrow>  K \<xi> \<rho>1 = K \<xi> \<rho>2)"
+apply (auto intro!: ext
+       arg_cong[of _ _ LAM] arg_cong[of _ _ AP] arg_cong2[of _ _ _ _ APP])
 apply (metis fun_upd_other fun_upd_twist)
 proof- (* todo: clean up proof *)
   fix x' x'a \<rho>1 \<rho>2 d assume "\<forall>y. y \<noteq> x' \<longrightarrow> \<rho>1 y = \<rho>2 y"
@@ -85,6 +86,150 @@ proof- (* todo: clean up proof *)
 qed
 
 end (* context Semantics *)
+
+(* Relativized depth, assuming weights for each (free) variable, is an
+  instance of the semantic-domain interpretation:  *)
+interpretation I : Semantics where APP = max and LAM = "\<lambda> K. Suc (K (0::nat))" done
+
+definition wdepth :: "('var,'const) trm \<Rightarrow> ('var \<Rightarrow> nat) \<Rightarrow> nat" where
+"wdepth X \<equiv> I.sem X (\<lambda> c. 0)"
+
+lemma wdepth_simps[simp]:
+  "wdepth (Var x) \<rho> = \<rho> x"
+  "wdepth (Ct c) \<rho> = 0"
+  "wdepth (App X Y) \<rho> = max (wdepth X \<rho>) (wdepth Y \<rho>)"
+  "wdepth (Lam x X) \<rho> = Suc (wdepth X (\<rho> (x := 0)))"
+  "wdepth (subst X Y y) \<rho> = wdepth X (\<rho> (y := wdepth Y \<rho>))"
+  "\<lbrakk>fresh x X; \<And> y. y \<noteq> x \<Longrightarrow>  \<rho>1 y = \<rho>2 y\<rbrakk> \<Longrightarrow>  wdepth X \<rho>1 = wdepth X \<rho>2"
+unfolding wdepth_def by auto
+
+(* The usual depth operator is obtained with weigth 0 for all variables: *)
+definition "depth X \<equiv> wdepth X (\<lambda> x. 0)"
+
+lemma depth_simps[simp]:
+  "depth (Var x) = 0"
+  "depth (Ct c) = 0"
+  "depth (App X Y) = max (depth X) (depth Y)"
+  "depth (Lam x X) = Suc (depth X)"
+unfolding depth_def by simp_all (metis fun_upd_triv)
+
+lemma depth_subst_var[simp]: "depth (subst X (Var z) x) = depth X"
+unfolding depth_def by simp (metis fun_upd_triv)
+
+(* Some setup: *)
+definition "isVar X \<equiv> \<exists> x. X = Var x"
+definition "isCt X \<equiv> \<exists> c. X = Ct c"
+definition "isApp X \<equiv> \<exists> X1 X2. X = App X1 X2"
+definition "isLam X \<equiv> \<exists> x X1. X = Lam x X1"
+definition "issubst X \<equiv> \<exists> X1 X2 x. X = subst X1 X2 x"
+
+lemma nchotomy_aux: "isVar X \<or> isCt X \<or> isApp X \<or> isLam X \<or> issubst X"
+apply(induction X) unfolding isVar_def isCt_def isApp_def isLam_def issubst_def by blast+
+
+lemma cases_aux:
+"\<lbrakk>isVar X \<Longrightarrow>  \<phi>; isCt X \<Longrightarrow>  \<phi>; isApp X \<Longrightarrow>  \<phi>; isLam X \<Longrightarrow>  \<phi>; issubst X \<Longrightarrow>  \<phi>\<rbrakk> \<Longrightarrow> \<phi>"
+using nchotomy_aux by auto
+
+lemma isVar_subst:
+assumes "isVar X1" shows "isVar (subst X1 X2 x) \<or> subst X1 X2 x = X2"
+proof-
+  obtain x1 where X1: "X1 = Var x1" using assms unfolding isVar_def by auto
+  show ?thesis unfolding isVar_def X1 by (cases "x = x1") auto
+qed
+
+lemma isCt_subst:
+assumes "isCt X1" shows "subst X1 X2 x = X1"
+using assms unfolding isCt_def by auto
+
+lemma isApp_subst:
+assumes "isApp X1" shows "isApp (subst X1 X2 x)"
+using assms unfolding isApp_def by fastforce
+
+lemma finite_nonFresh:
+fixes X :: "('var,'const) trm"
+assumes i: "\<not> finite (UNIV::'var set)" (* X :: "('var::infinite,'const) term" *)
+shows "finite {z. \<not> fresh z X}"
+proof (induction X)
+  fix x::'var
+  have "{z. \<not> fresh z (Var x)} \<subseteq> {x}" by (auto, case_tac "x = xa", auto)
+  thus "finite {z. \<not> fresh z (Var x)}" by (metis finite.simps subset_singletonD)
+next
+  fix c::'const show "finite {z::'var. \<not> fresh z (Ct c)}" using i by auto
+next
+  fix X1 X2 :: "('var,'const) trm"
+  assume "finite {z::'var. \<not> fresh z X1}" (is "finite ?A1")
+     and "finite {z::'var. \<not> fresh z X2}" (is "finite ?A2")
+  moreover have "{z::'var. \<not> fresh z (App X1 X2)} \<subseteq> ?A1 \<union> ?A2" (is "?B \<subseteq> _") by auto
+  ultimately show "finite ?B"
+  by (metis finite_UnI finite_subset)
+next
+  fix x :: 'var and X1 :: "('var,'const) trm"
+  assume "finite {z::'var. \<not> fresh z X1}" (is "finite ?A1")
+  moreover have "finite {x}" by simp
+  moreover have "{z::'var. \<not> fresh z (Lam x X1)} \<subseteq> ?A1 \<union> {x}" (is "?B \<subseteq> _") by auto
+  ultimately show "finite ?B" by (metis finite_UnI finite_subset)
+next
+  fix x :: 'var and X1 X2 :: "('var,'const) trm"
+  assume "finite {z::'var. \<not> fresh z X1}" (is "finite ?A1")
+     and "finite {z::'var. \<not> fresh z X2}" (is "finite ?A2")
+  moreover have "{z::'var. \<not> fresh z (subst X1 X2 x)} \<subseteq> ?A1 \<union> ?A2" (is "?B \<subseteq> _") by auto
+  ultimately show "finite ?B" by (metis finite_UnI finite_subset)
+qed
+
+lemma ex_fresh:
+fixes T :: "('var,'const) trm set"
+assumes i: "\<not> finite (UNIV::'var set)" (* X :: "('var::infinite,'const) term" *)
+and f: "finite A" and F: "finite T"
+shows "\<exists> z. (\<forall> X \<in> T. fresh z X) \<and> z \<notin> A"
+proof-
+  have "finite ((\<Union> X \<in> T. {z. \<not> fresh z X}) \<union> A)" (is "finite ?B")
+  using finite_nonFresh[OF i] f F by auto
+  hence "UNIV - ?B \<noteq> {}" by (metis finite.emptyI finite_Diff2 i)
+  thus ?thesis by auto
+qed
+
+lemma isLam_subst:
+fixes X :: "('var,'const) trm"
+assumes i: "\<not> finite (UNIV::'var set)" and "isLam X"
+shows "isLam (subst X X2 x)"
+proof-
+  obtain x1 X1 where X: "X = Lam x1 X1" using assms unfolding isLam_def by auto
+  then obtain y1 where y1: "fresh y1 X1" "fresh y1 X2" "y1 \<noteq> x1" "y1 \<noteq> x"
+  using ex_fresh[of "{x1,x}" "{X1,X2}", OF i] by auto
+  hence 1: "Lam x1 X1 = Lam y1 (subst X1 (Var y1) x1)" using subst_Lam by auto
+  show ?thesis unfolding X 1 isLam_def using y1 by (auto simp del: Lam_subst)
+qed
+
+(* A term is either a variable, or a constant, or an application, or an abstraction: *)
+lemma nchotomy:
+fixes X :: "('var,'const) trm"
+assumes i: "\<not> finite (UNIV::'var set)"
+shows "isVar X \<or> isCt X \<or> isApp X \<or> isLam X"
+proof (induction X)
+  fix x :: 'var and X1 X2 :: "('var,'const) trm"
+  assume X1: "isVar X1 \<or> isCt X1 \<or> isApp X1 \<or> isLam X1"
+  and X2: "isVar X2 \<or> isCt X2 \<or> isApp X2 \<or> isLam X2"
+  let ?Y = "subst X1 X2 x"
+  show "isVar ?Y \<or> isCt ?Y \<or> isApp ?Y \<or> isLam ?Y"
+  using X1 proof(elim disjE)
+    assume "isVar X1"
+    from isVar_subst[OF this, of X2 x] X2 show ?thesis by fastforce
+  qed (insert X1, auto simp: isCt_subst isApp_subst isLam_subst[OF i])
+qed (auto simp: isVar_def isCt_def isApp_def isLam_def)
+
+(* Picking fresh vars: *)
+definition pickFresh :: "(var,'const) trm list \<Rightarrow> var list \<Rightarrow> var"
+where "pickFresh Xs xs \<equiv> SOME x. (\<forall> X \<in> set Xs. fresh x X) \<and> x \<notin> set xs"
+
+lemma pickFresh:
+"(\<forall> X \<in> set Xs. fresh (pickFresh Xs xs) X) \<and> pickFresh Xs xs \<notin> set xs"
+unfolding pickFresh_def by (rule someI_ex, rule ex_fresh) auto
+
+lemma fresh_pickFresh[simp]: "X \<in> set Xs \<Longrightarrow>  fresh (pickFresh Xs xs) X"
+using pickFresh by auto
+
+lemma notIn_pickFresh[simp]: "pickFresh Xs xs \<notin> set xs"
+using pickFresh by auto
 
 
 
