LF.thy
@@ -1,0 +1,130 @@
+theory LF
+imports Prelim
+begin
+
+nonfreedata
+  ('ct, 'tct) obj =
+  Ct 'ct | Var var | Lam "('ct, 'tct) tfam" var "('ct, 'tct) obj" | App "('ct, 'tct) obj" "('ct, 'tct) obj"
+  | subst "('ct, 'tct) obj" "('ct, 'tct) obj" var
+and
+  ('ct, 'tct) tfam =
+  Tct 'tct | Tprod "('ct, 'tct) tfam" var "('ct, 'tct) tfam" | Tapp "('ct, 'tct) tfam" "('ct, 'tct) obj"
+  | tsubst "('ct, 'tct) tfam" "('ct, 'tct) obj" var
+and
+  ('ct, 'tct) kind = Type | Kprod "('ct, 'tct) tfam" var "('ct, 'tct) kind"
+  | ksubst "('ct, 'tct) kind" "('ct, 'tct) obj" var
+where
+  subst_Ct: "subst (Ct c) M x = Ct c"
+| subst_V1: "subst (Var x) M x = M"
+| subst_V2: "neq x y \<Longrightarrow> subst (Var x) N y = Var x"
+| subst_App: "subst (App M N) P x = App (subst M P x) (subst N P x)"
+| subst_Lam: "\<lbrakk>neq x y ; fresh x N\<rbrakk> \<Longrightarrow> subst (Lam A x M) N y = Lam (tsubst A N y) x (subst M N y)"
+| fresh_V: "neq x y \<Longrightarrow> fresh x (Var y)"
+| fresh_Ct: "fresh x (Ct c)"
+| fresh_App: "\<lbrakk>fresh x M; fresh x N\<rbrakk> \<Longrightarrow> fresh x (App M N)"
+| fresh_Lam1: "tfresh x A \<Longrightarrow> fresh x (Lam A x M)"
+| fresh_Lam2: "\<lbrakk>tfresh x A; fresh x M\<rbrakk> \<Longrightarrow> fresh x (Lam A y M)"
+| Lam_subst:  "\<lbrakk>neq y x ; fresh y M\<rbrakk> \<Longrightarrow> Lam A y (subst M (Var y) x) = Lam A x M"
+| fresh_subst: "\<lbrakk>fresh x M; fresh x N\<rbrakk> \<Longrightarrow>  fresh x (subst M N z)"
+(*  *)
+| tsubst_Tct: "tsubst (Tct a) M x = Tct a"
+| tsubst_Tapp: "tsubst (Tapp A N) M x = Tapp (tsubst A M x) (subst N M x)"
+| tsubst_Tprod: "\<lbrakk>neq x y ; fresh x N\<rbrakk> \<Longrightarrow> tsubst (Tprod A x B) N y = Tprod (tsubst A N y) x (tsubst B N y)"
+| tfresh_Tct: "tfresh x (Tct a)"
+| tfresh_Tapp: "\<lbrakk>tfresh x A; fresh x N\<rbrakk> \<Longrightarrow> tfresh x (Tapp A N)"
+| tfresh_Tprod1: "tfresh x A \<Longrightarrow> tfresh x (Tprod A x B)"
+| tfresh_Tprod2: "\<lbrakk>tfresh x A; tfresh x B\<rbrakk> \<Longrightarrow> tfresh x (Tprod A y B)"
+| Tprod_tsubst:  "\<lbrakk>neq y x ; tfresh y B\<rbrakk> \<Longrightarrow> Tprod A y (tsubst B (Var y) x) = Tprod A x B"
+| tfresh_tsubst: "\<lbrakk>tfresh x A; fresh x N\<rbrakk> \<Longrightarrow> tfresh x (tsubst A N z)"
+(*  *)
+| ksubst_Type: "ksubst Type M x = Type"
+| ksubst_Kprod: "\<lbrakk>neq x y ; fresh x N\<rbrakk> \<Longrightarrow> ksubst (Kprod A x K) N y = Kprod (tsubst A N y) x (ksubst K N y)"
+| kfresh_Type: "kfresh x Type"
+| kfresh_Kprod1: "tfresh x A \<Longrightarrow> kfresh x (Kprod A x K)"
+| kfresh_Kprod2: "\<lbrakk>tfresh x A; kfresh x K\<rbrakk> \<Longrightarrow> kfresh x (Kprod A y K)"
+| kfresh_ksubst: "\<lbrakk>kfresh x K; fresh x N\<rbrakk> \<Longrightarrow> kfresh x (ksubst K N z)"
+| Kprod_ksubst:  "\<lbrakk>neq y x ; kfresh y K\<rbrakk> \<Longrightarrow> Kprod A y (ksubst K (Var y) x) = Kprod A x K"
+
+declare subst_Ct[simp] subst_V1[simp] subst_V2[simp] subst_App[simp] subst_Lam[simp]
+fresh_Ct[simp] fresh_V[simp] fresh_App[simp] fresh_Lam1[simp] fresh_Lam2[simp]
+Lam_subst[simp] fresh_subst[simp]
+declare tsubst_Tct[simp] tsubst_Tapp[simp] tsubst_Tprod[simp]
+tfresh_Tct[simp] tfresh_Tapp[simp] tfresh_Tprod1[simp] tfresh_Tprod2[simp]
+Tprod_tsubst[simp] tfresh_tsubst[simp]
+
+declare ksubst_Type[simp] ksubst_Kprod[simp]
+kfresh_Type[simp] kfresh_Kprod1[simp] kfresh_Kprod2[simp]
+Kprod_ksubst[simp] kfresh_ksubst[simp]
+
+(* Unlike in Nominal and in my previous approach, terms do not have to be defined
+  mutually recursively with formulas just because formulas bind term variables *)
+datatype fterm = Fvar var | Sc fterm | Plus fterm fterm | Mult fterm fterm
+
+fun ftsubst where
+  "ftsubst (Fvar x) t y = (if x = y then t else Fvar x)"
+| "ftsubst (Sc s) t y = Sc (ftsubst s t y)"
+| "ftsubst (Plus s1 s2) t y = Plus (ftsubst s1 t y) (ftsubst s2 t y)"
+| "ftsubst (Mult s1 s2) t y = Mult (ftsubst s1 t y) (ftsubst s2 t y)"
+
+fun ftfresh where
+  "ftfresh z (Fvar x) \<longleftrightarrow> x \<noteq> z"
+| "ftfresh z (Sc s) \<longleftrightarrow> ftfresh z s"
+| "ftfresh z (Plus s1 s2) \<longleftrightarrow> ftfresh z s1 \<and> ftfresh z s2"
+| "ftfresh z (Mult s1 s2) \<longleftrightarrow> ftfresh z s1 \<and> ftfresh z s2"
+
+fun is_ftsubst where "is_ftsubst s t y s' = (ftsubst s t y = s')"
+fun is_Fvar where "is_Fvar t y = (t = Fvar y)"
+fun ftfreshFor where "ftfreshFor x y t = (neq x y \<and> ftfresh x t)"
+fun isFreshFvar where "isFreshFvar t y x = (is_Fvar t y \<and> neq y x)"
+
+nonfreedata
+  fmla = Eq fterm fterm | Leq fterm fterm | Neg fmla | Conj fmla fmla | All var fmla
+         | fsubst fmla fterm var
+where
+  fsubst_Eq: "\<lbrakk>is_ftsubst s1 t x s1'; is_ftsubst s2 t x s2'\<rbrakk>  \<Longrightarrow> fsubst (Eq s1 s2) t x = Eq s1' s2'"
+| fsubst_Leq: "\<lbrakk>is_ftsubst s1 t x s1'; is_ftsubst s2 t x s2'\<rbrakk>  \<Longrightarrow> fsubst (Leq s1 s2) t x = Leq s1' s2'"
+| subst_Neg: "fsubst (Neg f) t x = Neg (fsubst f t x)"
+| fsubst_Conj: "fsubst (Conj f1 f2) t x = Conj (fsubst f1 t x) (fsubst f2 t x)"
+| fsubst_All: "ftfreshFor x y t \<Longrightarrow> fsubst (All x f) t y = All x (fsubst f t y)"
+| ffresh_Eq: "\<lbrakk>ftfresh z s1; ftfresh z s2\<rbrakk> \<Longrightarrow> ffresh z (Eq s1 s2)"
+| ffresh_Leq: "\<lbrakk>ftfresh z s1; ftfresh z s2\<rbrakk> \<Longrightarrow> ffresh z (Leq s1 s2)"
+| ffresh_Neg: "ffresh x f \<Longrightarrow> ffresh x (Neg f)"
+| ffresh_Conj: "\<lbrakk>ffresh x f1; ffresh x f2\<rbrakk> \<Longrightarrow> ffresh x (Conj f1 f2)"
+| ffresh_All1: "ffresh x (All x f)"
+| ffresh_All2: "ffresh x f \<Longrightarrow> ffresh x (All y f)"
+| All_fsubst:  "\<lbrakk>isFreshFvar t y x  ; ffresh y f\<rbrakk> \<Longrightarrow> All y (fsubst f t x) = All x f"
+| ffresh_fsubst: "\<lbrakk>ffresh x f; ftfresh x t\<rbrakk> \<Longrightarrow>  ffresh x (fsubst f t z)"
+
+
+(* Representation: *)
+datatype tct = tm | fm
+datatype ct = sc | plus | times | eq | leq | neg | conj | all
+
+fun tenc :: "fterm \<Rightarrow> (ct,tct) obj"
+where
+  "tenc (Fvar x) = Var x"
+| "tenc (Sc t) = App (Ct sc) (tenc t)"
+| "tenc (Plus s t) = App (App (Ct plus) (tenc s)) (tenc t)"
+| "tenc (Mult s t) = App (App (Ct plus) (tenc s)) (tenc t)"
+
+lemma tenc_ftsubst[simp]: "tenc (ftsubst s t y) = subst (tenc s) (tenc t) y"
+by (induction s) auto
+
+lemma tenc_ftfresh[simp]: "ftfresh x t \<Longrightarrow> fresh x (tenc t)"
+by (induction t) auto
+
+(* Substitution-compositional interpetation of FOL syntax in LF: *)
+nonfreeiter
+  fenc :: "fmla \<Rightarrow> (ct,tct) obj"
+where
+  "fenc (Eq t1 t2) = App (App (Ct eq) (tenc t1)) (tenc t2)"
+| "fenc (Leq t1 t2) = App (App (Ct leq) (tenc t1)) (tenc t2)"
+| "fenc (Neg f) = App (Ct neg) (fenc f)"
+| "fenc (Conj f1 f2) = App (App (Ct conj) (fenc f1)) (fenc f2)"
+| "fenc (All x f) = App (Ct all) (Lam (Tct tm) x (fenc f))"
+| "fenc (fsubst f t y) = subst (fenc f) (tenc t) y"
+| "ffresh interpretedas (fresh :: var \<Rightarrow>  (ct,tct) obj \<Rightarrow> bool)"
+by auto
+
+
+end
