LF_to_STLC.thy
@@ -1,0 +1,166 @@
+(* The encoding of LF in Curry-style simply typed lambda calculus *)
+theory LF_to_STLC
+imports LF Terms_with_Bindings
+begin
+
+(* Simple types: *)
+datatype 'tct stype = Tp 'tct | Omega | Arr "'tct stype" "'tct stype"
+
+definition "unity u = ()"
+definition "unity2 u v = ()"
+
+nonfreeiter
+  otau :: "('ct,'tct) obj \<Rightarrow> unit"
+and
+  ftau :: "('ct,'tct) tfam \<Rightarrow> 'tct stype"
+and
+  ktau :: "('ct,'tct) kind \<Rightarrow> 'tct stype"
+where
+  "otau (LF.Ct c) = ()"
+| "otau (LF.Var x) = ()"
+| "otau (LF.Lam A x M) = unity2 (ftau A) (otau M)"
+| "otau (LF.App M N) = unity2 (otau M) (otau N)"
+| "otau (LF.subst M N x) = unity2 (otau M) (otau N)"
+(*  *)
+| "ftau (LF.Tct a) = Tp a"
+| "ftau (LF.Tprod A x B) = Arr (ftau A) (ftau B)"
+| "ftau (LF.Tapp A M) = fst (ftau A, otau M)"
+| "ftau (LF.tsubst A N x) = fst (ftau A, otau N)"
+(*  *)
+| "ktau Type = Omega"
+| "ktau (LF.Kprod A x K) = Arr (ftau A) (ktau K)"
+| "ktau (LF.ksubst K N x) = fst (ktau K, otau N)"
+(*  *)
+| "(LF.fresh :: var \<Rightarrow> ('ct,'tct) obj \<Rightarrow> bool)
+   interpretedas
+   (\<lambda> (x::var) (u::unit). True)"
+| "(LF.tfresh :: var \<Rightarrow> ('ct,'tct) tfam \<Rightarrow> bool)
+   interpretedas
+   (\<lambda> (x::var) (\<sigma>::'tct stype). True)"
+| "(LF.kfresh :: var \<Rightarrow> ('ct,'tct) kind \<Rightarrow> bool)
+   interpretedas
+   (\<lambda> (x::var) (\<sigma>::'tct stype). True)"
+by auto
+
+datatype ('ct,'tct) const = Pi "'tct stype" | LFconst 'ct | LFtconst 'tct
+
+
+lemma [simp]:
+assumes "x' \<noteq> x" and "fresh x' X" and
+y: "y = pickFresh [subst X (Var x') x] []" and z: "z = pickFresh [X] []"
+shows "Lam y (Lam x X) = Lam z (Lam x X)"
+sorry
+(* Proof: By "Lam y" and "Lam z" being dummy abstractions.  That "Lam y" is so
+follows from a property about fresh and subst.  *)
+
+lemma [simp]:
+assumes "x' \<noteq> x" and "fresh x' Y" and
+y: "y = pickFresh [X] []" and z: "z = pickFresh [subst X Y x] []"
+shows "subst (Lam y (Lam x' X)) Y x = Lam z (Lam x' (subst X Y x))"
+sorry
+(* Proof: Since above "Lam y" and "Lam z" are dummy abstractions, they can be replaced by some
+totally fresh u.  Now,  "subst (Lam u (Lam x' X)) Y x = Lam u (Lam x' (subst X Y x))"
+follows by appliying subst_lam twice.  *)
+
+
+(* The "modulus" operator: Since the package does not support full recursion,
+  I need to go through an auxiliary operator returning pairs (just like I did for the finite-set cardinal).
+  The only culprit is "ftau A" from the "LF.Tprod A x B" case. *)
+nonfreeiter
+  omod' :: "('ct,'tct) obj \<Rightarrow> ('ct,'tct) obj \<times> (var, ('ct,'tct) const) trm"
+and
+  fmod' :: "('ct,'tct) tfam \<Rightarrow> ('ct,'tct) tfam \<times> (var, ('ct,'tct) const) trm"
+and
+  kmod' :: "('ct,'tct) kind \<Rightarrow> unit"
+where
+  "omod' (LF.Ct c) = (LF.Ct c, Ct (LFconst c))"
+| "omod' (LF.Var x) = (LF.Var x, Var x)"
+| "omod' (LF.Lam A x M) =
+   (
+    case (fmod' A, omod' M) of ((A,X), (M,Y)) \<Rightarrow>
+     (LF.Lam A x M, App (Lam (pickFresh [Y] []) (Lam x (Y))) X)
+   )"
+| "omod' (LF.App M N) =
+   (case (omod' M, omod' N) of ((M,X), (N,Y)) \<Rightarrow>
+     (LF.App M N, App X Y)
+   )"
+| "omod' (LF.subst M N x) =
+   (case (omod' M, omod' N) of ((M,X), (N,Y)) \<Rightarrow>
+     (LF.subst M N x, subst X Y x)
+   )"
+(*  *)
+| "fmod' (LF.Tct a) = (LF.Tct a, Ct (LFtconst a))"
+| "fmod' (LF.Tprod A x B) =
+   (
+    case (fmod' A, fmod' B) of ((A,X), (B,Y)) \<Rightarrow>
+     (LF.Tprod A x B, App (App (Ct (Pi (ftau A))) X) (Lam x Y))
+   )"
+| "fmod' (LF.Tapp A M) =
+   (
+    case (fmod' A, omod' M) of ((A,X), (M,Y)) \<Rightarrow>
+     (LF.Tapp A M, App X Y)
+   )"
+| "fmod' (LF.tsubst A N x) =
+  (
+   case (fmod' A, omod' N) of ((A,X), (N,Y)) \<Rightarrow>
+    (LF.tsubst A N x, subst X Y x)
+  )"
+(*  *)
+| "kmod' Type = ()"
+| "kmod' (LF.Kprod A x K) = unity2 (fmod' A) (kmod' K)"
+| "kmod' (LF.ksubst K N x) = unity2 (kmod' K) (omod' N)"
+(*  *)
+| "(LF.fresh :: var \<Rightarrow> ('ct,'tct) obj \<Rightarrow> bool)
+   interpretedas
+   ((\<lambda> x (M,X). LF.fresh x M \<and> fresh x X) :: var \<Rightarrow> ('ct,'tct) obj \<times> (var, ('ct,'tct) const) trm \<Rightarrow> bool)"
+| "(LF.tfresh :: var \<Rightarrow> ('ct,'tct) tfam \<Rightarrow> bool)
+   interpretedas
+   ((\<lambda> x (A,X). LF.tfresh x A \<and> fresh x X) :: var \<Rightarrow> ('ct,'tct) tfam \<times> (var, ('ct,'tct) const) trm \<Rightarrow> bool)"
+| "(LF.kfresh :: var \<Rightarrow> ('ct,'tct) kind \<Rightarrow> bool)
+   interpretedas
+   (\<lambda> (x::var) (u::unit). True)"
+by auto
+
+lemma fst_omod'[simp]: "fst (omod' M) = M"
+apply(induction rule: obj_induct[of "\<lambda> A. fst (fmod' A) = A" "\<lambda> M. fst (omod' M) = M"])
+by (auto split: prod.splits)
+
+lemma omod'_Pair: "omod' M = (M',X) \<Longrightarrow> M = M'"
+using fst_omod' by (metis fst_conv)
+
+lemma fst_fmod'[simp]: "fst (fmod' A) = A"
+apply(induction rule: tfam_induct[of "\<lambda> A. fst (fmod' A) = A" "\<lambda> M. fst (omod' M) = M"]) apply auto
+by (auto split: prod.splits dest: omod'_Pair)
+
+lemma fmod'_Pair: "fmod' A = (A',X) \<Longrightarrow> A = A'"
+using fst_fmod' by (metis fst_conv)
+
+definition "omod \<equiv> snd o omod'"
+definition "fmod \<equiv> snd o fmod'"
+
+lemma mod_simps[simp]:
+"omod (LF.Ct c) = Ct (LFconst c)"
+"omod (LF.Var x) = Var x"
+"omod (LF.Lam A x M) = App (Lam (pickFresh [omod M] [])
+                           (Lam x (omod M))) (fmod A)"
+"omod (LF.App M N) = App (omod M) (omod N)"
+(*  *)
+"fmod (LF.Tct a) = Ct (LFtconst a)"
+"fmod (LF.Tprod A x B) = App (App (Ct (Pi (ftau A))) (fmod A)) (Lam x (fmod B))"
+"fmod (LF.Tapp A M) = App (fmod A) (omod M)"
+unfolding omod_def fmod_def by (auto split: prod.split dest: fmod'_Pair)
+
+lemma mod_subst[simp]:
+"omod (LF.subst M N x) = subst (omod M) (omod N) x"
+"fmod (LF.tsubst A N x) = subst (fmod A) (omod N) x"
+unfolding omod_def fmod_def by (auto split: prod.splits)
+
+lemma mod_fresh[simp]:
+"LF.fresh x M \<Longrightarrow> fresh x (omod M)"
+"LF.tfresh x A \<Longrightarrow> fresh x (fmod A)"
+unfolding omod_def fmod_def apply (auto split: prod.splits)
+by (smt kmod'.simps split_conv surjective_pairing)+
+
+
+
+end
