Prelim.thy
@@ -1,0 +1,12 @@
+theory Prelim
+imports NonFree
+uses "input.ML"
+begin
+
+type_synonym var = nat
+
+fun neq where "neq x y = (x \<noteq> y)"
+hide_const app hide_const App hide_const Var
+
+
+end
